expand classical properties

theories/TraceClassicalProperties.v
@@ -1,4 +1,4 @@
-From Coq Require Import Classical.
+From Coq Require Import Classical ClassicalEpsilon.
 From CoindTraces Require Import SsrExport Traces TraceProperties.
 
 Set Implicit Arguments.
@@ -10,13 +10,13 @@ Section TraceClassicalProperties.
 Context {A B : Type}.
 
 Local Notation trace := (@trace A B).
+Local Notation propT := (@propT A B).
 
 Lemma not_infiniteT_finiteT : forall tr : trace,
  ~ infiniteT tr -> finiteT tr.
 Proof.
 move => tr Hnot.
-pose proof (classic (finiteT tr)) as Hinf.
-case: Hinf => Hinf //.
+case (classic (finiteT tr)) => Hinf //.
 case: Hnot.
 exact: not_finiteT_infiniteT.
 Qed.
@@ -25,10 +25,52 @@ Lemma finiteT_infiniteT : forall tr : trace,
  finiteT tr \/ infiniteT tr.
 Proof.
 move => tr.
-pose proof (classic (finiteT tr)) as Hinf.
-case: Hinf => Hinf; first by left.
+case (classic (finiteT tr)) => Hinf; first by left.
 right.
 exact: not_finiteT_infiniteT.
+Qed.
+
+CoFixpoint midp (p0 p1: trace -> Prop) tr0 tr1 (h: followsT (appendT p0 p1) tr0 tr1) : trace.
+Proof.
+case (followsT_dec h).
+- case => tr; case => st; case => h1; case => h2 h3.
+  apply constructive_indefinite_description in h3.
+  case: h3 => x [h4 h5].
+  apply x.
+- case => tr; case => tr'. case => a; case => b; case => h1; case => h2 h3.
+  apply (Tcons a b (@midp _ _ _ _ h3)).
+Defined.
+
+Lemma midpointT_midp : forall (p0 p1: trace -> Prop)  tr0 tr1 (h : followsT (appendT p0 p1) tr0 tr1),
+ midpointT h (midp h).
+Proof.
+cofix CIH.
+dependent inversion h.
+- subst.
+  intros.
+  rewrite [midp _]trace_destr. simpl.
+  case (constructive_indefinite_description _ _); simpl.
+  move => x [a1 hm].
+  by apply midpointT_nil => //; destruct x.
+- subst.
+  rewrite [midp _]trace_destr. simpl.
+  by apply (@midpointT_delay _ _ p0 p1 (Tcons a b tr) (Tcons a b tr') (followsT_delay a b f) tr tr' f a b (midp f)).
+Qed.
+
+Lemma appendT_assoc_R: forall p1 p2 p3,
+ forall tr : trace, (appendT p1 (appendT p2 p3)) tr -> (appendT (appendT p1 p2)  p3) tr.
+Proof.
+move => p1 p2 p3 tr0 h1.  move: h1 => [tr1 [h1 h2]].
+exists (midp h2). split.
+- exists tr1; split => //.
+  exact: (midpointT_before (midpointT_midp h2)).
+- exact: (midpointT_after (midpointT_midp h2)).
+Qed.
+
+Lemma AppendT_assoc_R: forall (p1 p2 p3 : propT), (p1 *** p2 *** p3) =>> (p1 *** p2) *** p3.
+Proof.
+move => p1 p2 p3 tr0 h1. destruct p1 as [f1 hf1]. destruct p2 as [f2 hf2].
+destruct p3 as [f3 hf3]. simpl. simpl in h1. apply appendT_assoc_R. by apply h1.
 Qed.
 
 End TraceClassicalProperties.
